Strong correctness and termination of JumpTarget

TM/LM/JumpTargetTM.v
@@ -1,21 +1,10 @@
-Require Import HeapTM.
-Require Import MatchList.
-Require Import ListTM.
+Require Import TM.Code.ProgrammingTools.
+Require Import TM.LM.Semantics TM.LM.Alphabets.
+Require Import TM.LM.MatchTok.
+Require Import TM.Code.ListTM TM.Code.MatchList TM.Code.MatchNat.
 
 Local Arguments plus : simpl never.
 Local Arguments mult : simpl never.
-
-Fixpoint jumpTarget (k:nat) (Q:Pro) (P:Pro) : option (Pro*Pro) :=
-  match P with
-  | retT :: P' => match k with
-                 | 0 => Some (Q,P')
-                 | S k' => jumpTarget k' (Q++[retT]) P'
-                 end
-  | lamT :: P' => jumpTarget (S k) (Q++[lamT]) P'
-  | t :: P' => jumpTarget k (Q++[t]) P' (* either [varT n] or [appT] *)
-  | [] => None
-  end.
-
 
 (** The [JumpTarget] machine only operates on programs. Consequently, the alphabet of [JumpTarget] is just [sigPro]. [JumpTarget] will also assume, that the result of [jumpTarget] is [Some]. *)
 
@@ -74,7 +63,7 @@ Proof.
     exists (Q++Q'), Q. repeat split; eauto.
   }
 Qed.
-    
+
 
 (** append a token to the token list *)
 Definition App_ATok (t : ATok) : pTM sigPro^+ (FinType(EqType unit)) 2 :=
@@ -173,7 +162,7 @@ Proof.
     - apply Reset_Terminates with (X := Tok).
   }
   {
-    intros tin k (Q&t&HEncQ&HEncT&HRight&Hk). unfold App_Tok_steps in Hk. 
+    intros tin k (Q&t&HEncQ&HEncT&HRight&Hk). unfold App_Tok_steps in Hk.
     exists (Constr_nil_steps), (1 + Constr_cons_steps _ t + 1 + App_Tokens_steps Q [t] + Reset_steps _ t). cbn. repeat split; try omega.
     intros tmid () (HNil&HInjNil); TMSimp. modpon HNil.
     exists (Constr_cons_steps _ t), (1 + App_Tokens_steps Q [t] + Reset_steps _ t). cbn. repeat split; try omega.
@@ -188,64 +177,70 @@ Qed.
 
 
 
-Definition JumpTarget_Step : pTM sigPro^+ (FinType(EqType (bool*unit))) 5 :=
-  Inject (MatchList sigTok_fin) [|Fin0; Fin3|];;
-  MATCH (Inject (ChangeAlphabet MatchTok _) [|Fin3|])
-         (fun t : option ATok =>
-            match t with
-            | Some retAT =>
-              If (MatchNat ⇑ retr_nat_prog @ [|Fin2|])
-                 (Return (App_ATok retAT @ [|Fin1; Fin4|]) (true, tt)) (* continue *)
-                 (Nop (false, tt)) (* return *)
-            | Some lamAT =>
-              Return (Constr_S ⇑ retr_nat_prog @ [|Fin2|];;
-                      App_ATok lamAT @ [|Fin1; Fin4|])
-                     (true,default) (* continue *)
-            | Some appAT =>
-              Return (App_ATok appAT @ [|Fin1;Fin4|])
-                     (true,default) (* continue *)
-            | None => (* Variable *)
-              Return (Constr_varT ⇑ _ @ [|Fin3|];;
-                      App_Tok @ [|Fin1; Fin3; Fin4|])
-                     (true,default) (* continue *)
-            end)
+Definition JumpTarget_Step : pTM sigPro^+ (option bool) 5 :=
+  If (Inject (MatchList sigTok_fin) [|Fin0; Fin3|])
+     (MATCH (Inject (ChangeAlphabet MatchTok _) [|Fin3|])
+             (fun t : option ATok =>
+                match t with
+                | Some retAT =>
+                  If (MatchNat ⇑ retr_nat_prog @ [|Fin2|])
+                     (Return (App_ATok retAT @ [|Fin1; Fin4|]) None) (* continue *)
+                     (Nop (Some true)) (* return true *)
+                | Some lamAT =>
+                  Return (Constr_S ⇑ retr_nat_prog @ [|Fin2|];;
+                          App_ATok lamAT @ [|Fin1; Fin4|])
+                         None (* continue *)
+                | Some appAT =>
+                  Return (App_ATok appAT @ [|Fin1;Fin4|])
+                         None (* continue *)
+                | None => (* Variable *)
+                  Return (Constr_varT ⇑ _ @ [|Fin3|];;
+                          App_Tok @ [|Fin1; Fin3; Fin4|])
+                         None (* continue *)
+                end))
+     (Nop (Some false)) (* return false *)
 .
 
 
-Definition JumpTarget_Step_Rel : pRel sigPro^+ (FinType(EqType(bool*unit))) 5 :=
-  ignoreSecond (
-      fun tin '(yout, tout) =>
-        forall (P Q : Pro) (k : nat) (t : Tok),
-          tin[@Fin0] ≃ t :: P ->
-          tin[@Fin1] ≃ Q ->
-          tin[@Fin2] ≃ k ->
-          isRight tin[@Fin3] -> isRight tin[@Fin4] ->
-          match yout, t with
-          | _, retT =>
-            match yout, k with
-            | false, O => (* return *)
-              tout[@Fin0] ≃ P /\
-              tout[@Fin1] ≃ Q /\
-              tout[@Fin2] ≃ 0
-            | true, S k' => (* continue *)
-              tout[@Fin0] ≃ P /\
-              tout[@Fin1] ≃ Q ++ [retT] /\
-              tout[@Fin2] ≃ k'
-            | _, _ => False (* not the case *)
-            end
-          | true, lamT => (* continue *)
-            tout[@Fin0] ≃ P /\
-            tout[@Fin1] ≃ Q ++ [lamT] /\
-            tout[@Fin2] ≃ S k
-          | true, t => (* continue *)
-            tout[@Fin0] ≃ P /\
-            tout[@Fin1] ≃ Q ++ [t] /\
-            tout[@Fin2] ≃ k
-          | _, _ => False (* not the case *)
-          end /\
-          isRight tout[@Fin3] /\
-          isRight tout[@Fin4]
-    ).
+Definition JumpTarget_Step_Rel : pRel sigPro^+ (option bool) 5 :=
+  fun tin '(yout, tout) =>
+    forall (P Q : Pro) (k : nat),
+      tin[@Fin0] ≃ P ->
+      tin[@Fin1] ≃ Q ->
+      tin[@Fin2] ≃ k ->
+      isRight tin[@Fin3] -> isRight tin[@Fin4] ->
+      match yout, P with
+      | _, retT :: P =>
+        match yout, k with
+        | Some true, O => (* return true *)
+          tout[@Fin0] ≃ P /\
+          tout[@Fin1] ≃ Q /\
+          tout[@Fin2] ≃ 0
+        | None, S k' => (* continue *)
+          tout[@Fin0] ≃ P /\
+          tout[@Fin1] ≃ Q ++ [retT] /\
+          tout[@Fin2] ≃ k'
+        | _, _ => False (* not the case *)
+        end
+      | None, lamT :: P => (* continue *)
+        tout[@Fin0] ≃ P /\
+        tout[@Fin1] ≃ Q ++ [lamT] /\
+        tout[@Fin2] ≃ S k
+      | None, t :: P => (* continue *)
+        tout[@Fin0] ≃ P /\
+        tout[@Fin1] ≃ Q ++ [t] /\
+        tout[@Fin2] ≃ k
+      | Some false, nil => (* return false *)
+        (*
+        tout[@Fin0] ≃ nil /\
+        tout[@Fin1] ≃ Q /\
+        tout[@Fin2] ≃ k
+         *)
+        True
+      | _, _ => False (* not the case *)
+      end /\
+      isRight tout[@Fin3] /\
+      isRight tout[@Fin4].
 
 
 Lemma JumpTarget_Step_Realise : JumpTarget_Step ⊨ JumpTarget_Step_Rel.
@@ -260,47 +255,49 @@ Proof.
     - apply App_Tok_Realise.
   }
   {
-    intros tin ((yout, ()), tout) H. cbn. intros P Q k t HEncP HEncQ HEncK HInt3 HInt4.
-    unfold sigPro in *. TMSimp. rename H into HMatchList, H0 into HMatchTok, H1 into HCase.
-    modpon HMatchList. destruct ymid; auto; modpon HMatchList.
-    modpon HMatchTok.
-    destruct ymid0 as [ [ | | ] | ]; try destruct t; auto; simpl_surject; TMSimp.
-    { (* t = retT *)
-      destruct HCase; TMSimp.
-      { (* k = S k' *) rename H into HMatchNat, H0 into HReturn, H1 into HApp.
-        modpon HMatchNat. destruct k as [ | k']; auto; modpon HMatchNat.
-        inv HReturn.
+    intros tin (yout, tout) H. cbn. intros P Q k HEncP HEncQ HEncK HInt3 HInt4.
+    unfold sigPro in *. rename H into HIf.
+    destruct HIf; TMSimp.
+    { (* Then of [MatchList], i.e. P = t :: P' *) rename H into HMatchList, H0 into HMatchTok, H1 into HCase.
+      modpon HMatchList. destruct P as [ | t P']; auto; modpon HMatchList.
+      modpon HMatchTok.
+      destruct ymid as [ [ | | ] | ]; try destruct t; auto; simpl_surject; TMSimp.
+      { (* t = retT *)
+        destruct HCase; TMSimp.
+        { (* k = S k' *) rename H into HMatchNat, H0 into HApp.
+          modpon HMatchNat. destruct k as [ | k']; auto; modpon HMatchNat.
+          modpon HApp.
+          repeat split; auto.
+        }
+        { (* k = 0 *) rename H into HMatchNat.
+          modpon HMatchNat. destruct k as [ | k']; auto; modpon HMatchNat.
+          repeat split; auto.
+        }
+      }
+      { (* t = lamT *) rename H into HS, H0 into HApp.
+        modpon HS.
         modpon HApp.
         repeat split; auto.
       }
-      { (* k = 0 *) rename H into HMatchNat, H0 into HReturn.
-        modpon HMatchNat. destruct k as [ | k']; auto; modpon HMatchNat.
-        inv HReturn.
+      { (* t = appT *) rename H into HApp.
+        modpon HApp.
+        repeat split; auto.
+      }
+      { (* t = varT *) rename H into HVar, H0 into HApp.
+        modpon HVar.
+        modpon HApp.
         repeat split; auto.
       }
     }
-    { (* t = lamT *) rename H into HReturn, H0 into HS, H1 into HApp.
-      inv HReturn.
-      modpon HS.
-      modpon HApp.
-      repeat split; auto.
-    }
-    { (* t = appT *) rename H into HReturn, H0 into HApp.
-      inv HReturn.
-      modpon HApp.
-      repeat split; auto.
-    }
-    { (* t = varT *) rename H into HReturn, H0 into HVar, H1 into HApp.
-      inv HReturn.
-      modpon HVar.
-      modpon HApp.
-      repeat split; auto.
+    { (* Else of [MatchList], i.e. P = nil *)
+      modpon H. destruct P; auto; modpon H; auto.
     }
   }
 Qed.
 
 
-Definition JumpTarget_Step_steps' (Q: Pro) (k: nat) (t: Tok) :=
+(* Steps after the [MatchTok], depending on [t] *)
+Local Definition JumpTarget_Step_steps_MatchTok (Q: Pro) (k: nat) (t: Tok) :=
   match t with
   | retT =>
     match k with
@@ -312,17 +309,26 @@ Definition JumpTarget_Step_steps' (Q: Pro) (k: nat) (t: Tok) :=
   | varT n => 1 + Constr_varT_steps + App_Tok_steps Q t
   end.
 
-Definition JumpTarget_Step_steps (Q: Pro) (k: nat) (t: Tok) :=
-  2 + MatchList_steps_cons _ t + MatchTok_steps + JumpTarget_Step_steps' Q k t.
+(* Steps after the [MatchList] *)
+Local Definition JumpTarget_Step_steps_MatchList (P Q : Pro) (k: nat) :=
+  match P with
+  | t :: P' => 1 + MatchTok_steps + JumpTarget_Step_steps_MatchTok Q k t
+  | nil => 0
+  end.
+
+(* Total steps *)
+Definition JumpTarget_Step_steps (P Q: Pro) (k: nat) :=
+  1 + MatchList_steps _ P + JumpTarget_Step_steps_MatchList P Q k.
+
 
 Definition JumpTarget_Step_T : tRel sigPro^+ 5 :=
   fun tin steps => (* Warning: I have to use another variable for the steps, since [k] is used. *)
-    exists (P Q : Pro) (k : nat) (t : Tok),
-      tin[@Fin0] ≃ t :: P /\
+    exists (P Q : Pro) (k : nat),
+      tin[@Fin0] ≃ P /\
       tin[@Fin1] ≃ Q /\
       tin[@Fin2] ≃ k /\
       isRight tin[@Fin3] /\ isRight tin[@Fin4] /\
-      JumpTarget_Step_steps Q k t <= steps.
+      JumpTarget_Step_steps P Q k <= steps.
 
 Lemma JumpTarget_Step_Terminates : projT1 JumpTarget_Step ↓ JumpTarget_Step_T.
 Proof.
@@ -338,31 +344,34 @@ Proof.
     - apply App_Tok_Terminates.
   }
   {
-    intros tin steps (P&Q&k&t&HEncP&HEncQ&HEncK&HRight3&HRight4&Hk). unfold JumpTarget_Step_steps in Hk. cbn in *.
+    intros tin steps (P&Q&k&HEncP&HEncQ&HEncK&HRight3&HRight4&Hk). unfold JumpTarget_Step_steps in Hk. cbn in *.
     unfold sigPro in *.
-    exists (MatchList_steps _ (t::P)), (1 + MatchTok_steps + JumpTarget_Step_steps' Q k t). cbn; repeat split; try omega. eauto.
-    intros tmid bmatchlist (HMatchList&HMatchListInj); TMSimp. modpon HMatchList. destruct bmatchlist; auto; modpon HMatchList.
-    exists (MatchTok_steps), (JumpTarget_Step_steps' Q k t). cbn; repeat split; try omega.
-    intros tmid1 ytok (HMatchTok&HMatchTokInj); TMSimp. modpon HMatchTok.
-    destruct ytok as [ [ | | ] | ]; destruct t; auto; simpl_surject; TMSimp.
-    { (* t = retT *)
-      exists MatchNat_steps.
-      destruct k as [ | k'].
-      - (* k = 0 *)
-        exists 0. repeat split; try omega.
-        intros tmid2 bMatchNat (HMatchNat&HMatchNatInj); TMSimp. modpon HMatchNat. destruct bMatchNat; auto.
-      - (* k = S k' *)
-        exists (App_ATok_steps Q retAT). repeat split; try omega.
-        intros tmid2 bMatchNat (HMatchNat&HMatchNatInj); TMSimp. modpon HMatchNat. destruct bMatchNat; auto. hnf; cbn. eauto.
-    }
-    { (* t = lamT *)
-      exists (Constr_S_steps), (App_ATok_steps Q lamAT). repeat split; try omega.
-      intros tmid2 () (HS&HSInj); TMSimp. modpon HS. hnf; cbn. eauto.
-    }
-    { (* t = appT *) hnf; cbn; eauto. }
-    { (* t = varT n *)
-      exists (Constr_varT_steps), (App_Tok_steps Q (varT n)). repeat split; try omega.
-      intros tmid2 H (HVarT&HVarTInj); TMSimp. modpon HVarT. hnf; cbn. eauto 6.
+    exists (MatchList_steps _ P), (JumpTarget_Step_steps_MatchList P Q k). cbn; repeat split; try omega. eauto.
+    intros tmid bmatchlist (HMatchList&HMatchListInj); TMSimp. modpon HMatchList.
+    destruct bmatchlist, P as [ | t P']; auto; modpon HMatchList.
+    { (* P = t :: P' (* other case is done by auto *) *)
+      exists (MatchTok_steps), (JumpTarget_Step_steps_MatchTok Q k t). cbn; repeat split; try omega.
+      intros tmid1 ytok (HMatchTok&HMatchTokInj); TMSimp. modpon HMatchTok.
+      destruct ytok as [ [ | | ] | ]; destruct t; auto; simpl_surject; TMSimp.
+      { (* t = retT *)
+        exists MatchNat_steps.
+        destruct k as [ | k'].
+        - (* k = 0 *)
+          exists 0. repeat split; try omega.
+          intros tmid2 bMatchNat (HMatchNat&HMatchNatInj); TMSimp. modpon HMatchNat. destruct bMatchNat; auto.
+        - (* k = S k' *)
+          exists (App_ATok_steps Q retAT). repeat split; try omega.
+          intros tmid2 bMatchNat (HMatchNat&HMatchNatInj); TMSimp. modpon HMatchNat. destruct bMatchNat; auto. hnf; cbn. eauto.
+      }
+      { (* t = lamT *)
+        exists (Constr_S_steps), (App_ATok_steps Q lamAT). repeat split; try omega.
+        intros tmid2 () (HS&HSInj); TMSimp. modpon HS. hnf; cbn. eauto.
+      }
+      { (* t = appT *) hnf; cbn; eauto. }
+      { (* t = varT n *)
+        exists (Constr_varT_steps), (App_Tok_steps Q (varT n)). repeat split; try omega.
+        intros tmid2 H (HVarT&HVarTInj); TMSimp. modpon HVarT. hnf; cbn. eauto 6.
+      }
     }
   }
 Qed.
@@ -384,18 +393,25 @@ Fixpoint jumpTarget_k (k:nat) (Q:Pro) (P:Pro) : nat :=
 Definition JumpTarget_Loop := WHILE JumpTarget_Step.
 
 
-Definition JumpTarget_Loop_Rel : pRel sigPro^+ (FinType(EqType unit)) 5 :=
+Definition JumpTarget_Loop_Rel : pRel sigPro^+ bool 5 :=
   fun tin '(yout, tout) =>
-    forall (P Q : Pro) (k : nat) (P' Q' : Pro),
-      jumpTarget k Q P = Some (Q', P') ->
+    forall (P Q : Pro) (k : nat),
       tin[@Fin0] ≃ P ->
       tin[@Fin1] ≃ Q ->
       tin[@Fin2] ≃ k ->
       isRight tin[@Fin3] -> isRight tin[@Fin4] ->
-      tout[@Fin0] ≃ P' /\
-      tout[@Fin1] ≃ Q' /\
-      tout[@Fin2] ≃ jumpTarget_k k Q P /\
-      isRight tout[@Fin3] /\ isRight tout[@Fin4].
+      match yout with
+      | true =>
+        exists (P' Q' : Pro),
+        jumpTarget k Q P = Some (Q', P') /\
+        tout[@Fin0] ≃ P' /\
+        tout[@Fin1] ≃ Q' /\
+        tout[@Fin2] ≃ jumpTarget_k k Q P /\
+        isRight tout[@Fin3] /\ isRight tout[@Fin4]
+      | false =>
+        jumpTarget k Q P = None
+      end.
+
 
 
 
@@ -406,62 +422,42 @@ Proof.
     - apply JumpTarget_Step_Realise.
   }
   {
-    apply WhileInduction; intros; intros P Q k P' Q' HJumpSome HEncP HEncQ HEncK HRight3 HRight4; cbn in *.
+    apply WhileInduction; intros; intros P Q k HEncP HEncQ HEncK HRight3 HRight4; cbn in *.
     {
-      destruct P as [ | t P]; cbn in *; try congruence.
-      modpon HLastStep.
-      destruct t; auto. destruct k; auto; modpon HLastStep. inv HJumpSome.
-      repeat split; auto.
+      modpon HLastStep. destruct yout, P as [ | [ | | | ] P']; auto. destruct k; auto. modpon HLastStep.
+      cbn. eauto 10.
     }
     {
-      destruct P as [ | t P]; cbn in *; try congruence.
       modpon HStar.
-      destruct t; modpon HStar.
-      - (* t = varT *) modpon HLastStep. repeat split; auto.
-      - (* t = appT *) modpon HLastStep. repeat split; auto.
-      - (* t = lamT *) modpon HLastStep. repeat split; auto.
-      - (* t = varT k, k must be S k'*)
-        destruct k as [ | k']; auto; modpon HStar.
-        modpon HLastStep.
-        repeat split; auto.
+      destruct P as [ | [ | | | ] P']; auto; modpon HStar.
+      - (* P = varT n :: P' *) modpon HLastStep. destruct yout; auto.
+      - (* P = appT :: P' *) modpon HLastStep. destruct yout; auto.
+      - (* P = lamT :: P' *) modpon HLastStep. destruct yout; auto.
+      - (* P = varT k :: P', k = S k' *) destruct k as [ | k']; auto; modpon HStar. modpon HLastStep. destruct yout; auto.
     }
   }
 Qed.
 
-(*
-  match t with
-  | retT =>
-    match k with
-    | S _ => 1 + MatchNat_steps + App_ATok_steps Q retAT
-    | 0 => 1 + MatchNat_steps
-    end
-  | lamT => 1 + Constr_S_steps + App_ATok_steps Q lamAT
-  | appT => App_ATok_steps Q appAT
-  | varT n => 1 + Constr_varT_steps + App_Tok_steps Q t
-  end.
-*)
-
 
 Fixpoint JumpTarget_Loop_steps (P Q: Pro) (k: nat) : nat :=
   match P with
-  | nil => 0 (* underspecified *)
+  | nil => JumpTarget_Step_steps P Q k
   | t :: P' =>
     match t with
     | retT =>
       match k with
-      | S k' => 1 + JumpTarget_Step_steps Q k t + JumpTarget_Loop_steps P' (Q++[t]) k'
-      | 0 =>        JumpTarget_Step_steps Q k retT (* terminal case *)
+      | S k' => 1 + JumpTarget_Step_steps P Q k + JumpTarget_Loop_steps P' (Q++[t]) k'
+      | 0 =>        JumpTarget_Step_steps P Q k (* terminal case *)
       end
-    | lamT =>   1 + JumpTarget_Step_steps Q k t + JumpTarget_Loop_steps P' (Q++[t]) (S k)
-    | appT =>   1 + JumpTarget_Step_steps Q k t + JumpTarget_Loop_steps P' (Q++[t]) k
-    | varT n => 1 + JumpTarget_Step_steps Q k t + JumpTarget_Loop_steps P' (Q++[t]) k
+    | lamT =>   1 + JumpTarget_Step_steps P Q k + JumpTarget_Loop_steps P' (Q++[t]) (S k)
+    | appT =>   1 + JumpTarget_Step_steps P Q k + JumpTarget_Loop_steps P' (Q++[t]) k
+    | varT n => 1 + JumpTarget_Step_steps P Q k + JumpTarget_Loop_steps P' (Q++[t]) k
     end
   end.
 
 Definition JumpTarget_Loop_T : tRel sigPro^+ 5 :=
   fun tin steps =>
-    exists (P Q : Pro) (k : nat) (P' Q' : Pro),
-      jumpTarget k Q P = Some (Q', P') /\
+    exists (P Q : Pro) (k : nat),
       tin[@Fin0] ≃ P /\
       tin[@Fin1] ≃ Q /\
       tin[@Fin2] ≃ k /\
@@ -475,54 +471,66 @@ Proof.
   { apply JumpTarget_Step_Realise. }
   { apply JumpTarget_Step_Terminates. }
   {
-    intros tin steps. intros (P&Q&k&P'&Q'&HJump&HEncP&HEncQ&HEncK&HRight3&HRight4&Hk).
-    destruct P as [ | t P]; cbn in *. now inv HJump.
-    exists (JumpTarget_Step_steps Q k t). repeat split. hnf; cbn; eauto 10.
-    intros b () tmid HStep. modpon HStep. destruct b.
+    intros tin steps. intros (P&Q&k&HEncP&HEncQ&HEncK&HRight3&HRight4&Hk).
+    exists (JumpTarget_Step_steps P Q k). repeat split. hnf; cbn; eauto 10.
+    intros ymid tmid HStep. cbn in HStep. modpon HStep. destruct ymid as [ [ | ] | ].
+    { (* [Some true], i.e. [P = retT :: P'] and [k = 0] *)
+      destruct P as [ | [ | | | ] ]; auto. destruct k; auto.
+    }
+    { (* [Some false], i.e. [P = nil] *)
+      destruct P as [ | [ | | | ] ]; auto.
+    }
     { (* recursion cases *)
+      destruct P as [ | t P ]; auto.
       destruct t; modpon HStep.
       - (* t = varT n *)
         exists (JumpTarget_Loop_steps P (Q++[varT n]) k). split.
-        + hnf. do 5 eexists; repeat split; eauto.
+        + hnf. do 3 eexists; repeat split; eauto.
         + assumption.
       - (* t = appT *)
         exists (JumpTarget_Loop_steps P (Q++[appT]) k). split.
-        + hnf. do 5 eexists; repeat split; eauto.
+        + hnf. do 3 eexists; repeat split; eauto.
         + assumption.
       - (* t = lamT *)
         exists (JumpTarget_Loop_steps P (Q++[lamT]) (S k)). split.
-        + hnf. do 5 eexists; repeat split; eauto.
+        + hnf. do 3 eexists; repeat split; eauto.
         + assumption.
       - (* t = retT, k = S k' *)
         destruct k as [ | k']; auto; modpon HStep.
         exists (JumpTarget_Loop_steps P (Q++[retT]) k'). split.
-        + hnf. do 5 eexists; repeat split; eauto.
+        + hnf. do 3 eexists; repeat split; eauto.
         + assumption.
-    }
-    { (* termination case, i.e. t=retT and k=0 *)
-      destruct t; auto. destruct k; auto.
     }
   }
 Qed.
 
-                            
-Definition JumpTarget : pTM sigPro^+ unit 5 :=
+
+Definition JumpTarget : pTM sigPro^+ bool 5 :=
   WriteValue _ (@nil Tok) @ [|Fin1|];;
   WriteValue _ 0 @ [|Fin2|];;
-  JumpTarget_Loop;;
-  Reset _ @ [|Fin2|].
+  If (JumpTarget_Loop)
+     (Return (Reset _ @ [|Fin2|]) true)
+     (Nop false)
+.
 
 
-Definition JumpTarget_Rel : pRel sigPro^+ unit 5 :=
+Definition JumpTarget_Rel : pRel sigPro^+ bool 5 :=
   fun tin '(yout, tout) =>
-    forall (P : Pro) (P' Q' : Pro),
-      jumpTarget 0 nil P = Some (Q', P') ->
+    forall (P : Pro),
       tin[@Fin0] ≃ P ->
       isRight tin[@Fin1] ->
       (forall i : Fin.t 3, isRight tin[@FinR 2 i : Fin.t 5]) ->
-      tout[@Fin0] ≃ P' /\
-      tout[@Fin1] ≃ Q' /\
-      (forall i : Fin.t 3, isRight tout[@FinR 2 i : Fin.t 5]).
+      match yout with
+      | true =>
+        exists (P' Q' : Pro),
+        jumpTarget 0 nil P = Some (Q', P') /\
+        tout[@Fin0] ≃ P' /\
+        tout[@Fin1] ≃ Q' /\
+        (forall i : Fin.t 3, isRight tout[@FinR 2 i : Fin.t 5])
+      | false =>
+        jumpTarget 0 nil P = None
+      end.
+
 
 Lemma JumpTarget_Realise : JumpTarget ⊨ JumpTarget_Rel.
 Proof.
@@ -532,26 +540,36 @@ Proof.
     - apply Reset_Realise with (X := nat).
   }
   {
-    intros tin ((), tout) H. cbn. intros P P' Q' HJump HEncP HOut HInt.
-    TMSimp ( unfold sigPro, sigTok in * ).
-    rename H into HWriteNil, H0 into HWriteO, H1 into HLoop, H2 into HReset.
-    modpon HWriteNil.
-    modpon HWriteO.
-    modpon HLoop.
-    modpon HReset.
-    repeat split; auto. intros i; destruct_fin i; TMSimp_goal; auto.
+    intros tin (yout, tout) H. cbn. intros P HEncP HOut HInt.
+    TMSimp ( unfold sigPro, sigTok in * ). rename H into HWriteNil, H0 into HWriteO, H1 into HIf.
+    modpon HWriteNil. modpon HWriteO.
+    destruct HIf; TMSimp.
+    { (* Then, i.e. [jumpTarget k Q P = Some (Q', P') *) rename H into HLoop, H0 into HReset.
+      modpon HLoop. destruct HLoop as (P'&Q'&HLoop); modpon HLoop.
+      modpon HReset. do 2 eexists; repeat split; eauto. intros i; destruct_fin i; TMSimp_goal; auto.
+    }
+    { (* Else, i.e. [jumpTarget k Q P = None *)
+      now modpon H.
+    }
   }
 Qed.
 
 
+(* Steps after [JumpTarget_Loop] depend on the output of [JumpTarget_Loop]. *)
+Local Definition JumpTarget_steps_Loop (P : Pro) :=
+  match jumpTarget 0 nil P with
+  | None => 0 (* Nop *)
+  | Some _ => Reset_steps _ (jumpTarget_k 0 nil P)
+  end.
+
+
 Definition JumpTarget_steps (P : Pro) :=
-  3 + WriteValue_steps _ (@nil Tok) + WriteValue_steps _ 0 + JumpTarget_Loop_steps P nil 0 + Reset_steps _ (jumpTarget_k 0 nil P).
+  3 + WriteValue_steps _ (@nil Tok) + WriteValue_steps _ 0 + JumpTarget_Loop_steps P nil 0 + JumpTarget_steps_Loop P.
 
 
 Definition JumpTarget_T : tRel sigPro^+ 5 :=
   fun tin k =>
-    exists (P : Pro) (P' Q' : Pro),
-      jumpTarget 0 nil P = Some (Q', P') /\
+    exists (P : Pro),
       tin[@Fin0] ≃ P /\
       isRight tin[@Fin1] /\
       (forall i : Fin.t 3, isRight tin[@Fin.R 2 i]) /\
@@ -567,17 +585,20 @@ Proof.
     - apply Reset_Terminates with (X := nat).
   }
   {
-    intros tin k (P&P'&Q'&HJumpSome&HEncP&Hout&HInt&Hk). unfold JumpTarget_steps in Hk.
-    exists (WriteValue_steps _ (@nil Tok)), (1 + WriteValue_steps _ 0 + 1 + JumpTarget_Loop_steps P nil 0 + Reset_steps _ (jumpTarget_k 0 nil P)).
+    intros tin k (P&HEncP&Hout&HInt&Hk). unfold JumpTarget_steps in Hk.
+    exists (WriteValue_steps _ (@nil Tok)), (1 + WriteValue_steps _ 0 + 1 + JumpTarget_Loop_steps P nil 0 + JumpTarget_steps_Loop P).
     cbn; repeat split; try omega.
     intros tmid () (HWrite&HWriteInj); TMSimp. modpon HWrite.
-    exists (WriteValue_steps _ 0), (1 + JumpTarget_Loop_steps P nil 0 + Reset_steps _ (jumpTarget_k 0 nil P)).
+    exists (WriteValue_steps _ 0), (1 + JumpTarget_Loop_steps P nil 0 + JumpTarget_steps_Loop P).
     cbn; repeat split; try omega. now setoid_rewrite WriteValue_steps_comp. now rewrite Nat.add_assoc.
     unfold sigPro in *. intros tmid1 () (HWrite'&HWriteInj'); TMSimp. modpon HWrite'.
-    exists (JumpTarget_Loop_steps P nil 0), (Reset_steps _ (jumpTarget_k 0 nil P)).
+    exists (JumpTarget_Loop_steps P nil 0), (JumpTarget_steps_Loop P).
     TMSimp. cbn; repeat split; try omega. cbn in *.
-    { hnf. do 5 eexists; repeat split; unfold sigPro in *; unfold eqType_X in *; cbn in *; TMSimp_goal; eauto. }
-    intros tmid2 () HLoop. modpon HLoop.
-    eexists; repeat split; eauto. now setoid_rewrite Reset_steps_comp.
+    { hnf. do 3 eexists; repeat split; unfold sigPro in *; unfold eqType_X in *; cbn in *; TMSimp_goal; eauto. }
+    intros tmid2 ymid HLoop. modpon HLoop. destruct ymid.
+    - (* true *) destruct HLoop as (P'&Q'&HLoop); modpon HLoop. eexists; repeat split; eauto.
+      setoid_rewrite Reset_steps_comp.
+      unfold JumpTarget_steps_Loop. now rewrite HLoop.
+    - (* false *) omega.
   }
 Qed.
